update to coq 8.15

theories/metacoq_utils.v
@@ -1,12 +1,16 @@
-From Coq Require Import Strings.String ssreflect ssrbool ssrfun.
+From Coq Require Import ssreflect ssrbool ssrfun.
 From MetaCoq.Template Require Import All.
+
+
 
 
 (** Helper functions relying on MetaCoq *)
 
 (** [build_const [t1;..;tn] body] builds the term λ(_:t1)..(_:tn).body *)
-Fixpoint build_const (argtys: list term) body :=
-  List.fold_right (fun ty t => tLambda nAnon ty t) body argtys.
+Definition build_const (argtys: list term) body :=
+  List.fold_right
+    (fun ty t => tLambda (mkBindAnn nAnon Relevant) ty t)
+     body argtys.
 
 (** [mkApps_ctx t shift ctx] build the application of t to the ctx shifted by shift *)
 Definition mkApps_ctx (t:term) (shift:nat) (ctx:context) :=
@@ -17,7 +21,7 @@ Definition mkApps_ctx (t:term) (shift:nat) (ctx:context) :=
       | Some _ => args
       end
     in
-    utils.fold_left_i fold_fun ctx nil in
+    fold_left_i fold_fun ctx nil in
   mkApps t args.
 
 Definition is_prim_record (decl:mutual_inductive_body) : option (option ident)
@@ -25,83 +29,96 @@ Definition is_prim_record (decl:mutual_inductive_body) : option (option ident)
     match ind_bodies decl with
     | (oib :: nil)%list =>
       match ind_ctors oib with
-      | (((id,_), _) :: nil)%list => Some (Some id) (* Some data is missing wrt to primitivity *)
+      | (ctor_body :: nil)%list => Some (Some (cstr_name ctor_body)) (* Some data is missing wrt to primitivity *)
       | _ => None
       end
     | _ => None
     end.
 
+
+Definition one_ind_body_to_entry (decl : mutual_inductive_body) (oib : one_inductive_body) : one_inductive_entry :=
+  let ra := remove_arity decl.(ind_npars) in
+  let ctors := oib.(ind_ctors) in
+  {|
+    mind_entry_typename := oib.(ind_name);
+    mind_entry_arity :=  oib.(ind_type);
+    mind_entry_consnames := List.map cstr_name ctors ;
+    mind_entry_lc := List.map (fun x => ra x.(cstr_type)) ctors;
+  |}.
+
+Arguments List.combine {_ _} _ _.
+Definition mind_body_params (decl : mutual_inductive_body) : context :=
+  match List.hd_error decl.(ind_bodies) with
+  | Some oib =>
+      let args := fst (decompose_prod oib.(ind_type)) in
+      let nametypes := List.firstn decl.(ind_npars) (uncurry List.combine args) in
+      List.rev (List.map (uncurry vass) nametypes)
+  | None => nil
+  end.
+Arguments List.combine [_ _] _ _.
+
 Definition mind_body_to_entry (decl : mutual_inductive_body)
-  : mutual_inductive_entry.
-Proof.
-  refine {| mind_entry_record := is_prim_record decl;
-            mind_entry_finite := ind_finite decl;
-            mind_entry_params := _;
-            mind_entry_inds := _;
-            mind_entry_universes := decl.(ind_universes);
-            mind_entry_private := None |}.
-  - refine (match List.hd_error decl.(ind_bodies) with
-            | Some i0 => List.rev _
-            | None => nil (* assert false: at least one inductive in a mutual block *)
-            end).
-    have [[names types] _] := decompose_prod i0.(ind_type).
-    apply (List.firstn decl.(ind_npars)) in names.
-    apply (List.firstn decl.(ind_npars)) in types.
-    apply: List.combine; [
-      exact (List.map get_ident names)
-    | exact (List.map LocalAssum types)].
-  - refine (List.map _ decl.(ind_bodies)).
-    intros [].
-    refine {| mind_entry_typename := ind_name;
-              mind_entry_arity := remove_arity decl.(ind_npars) ind_type;
-              mind_entry_template := false;
-              mind_entry_consnames := _;
-              mind_entry_lc := _;
-            |}.
-    exact (List.map (fun x => fst (fst x)) ind_ctors).
-    exact (List.map (fun x => remove_arity decl.(ind_npars)
-                                                (snd (fst x))) ind_ctors).
-Defined.
+  : mutual_inductive_entry :=
+  {|
+    mind_entry_record := is_prim_record decl;
+    mind_entry_finite := ind_finite decl;
+    mind_entry_params := mind_body_params decl ;
+    mind_entry_inds := List.map (one_ind_body_to_entry decl) decl.(ind_bodies);
+    mind_entry_universes := Universes.universes_entry_of_decl decl.(ind_universes);
+    mind_entry_private := None ;
+    mind_entry_template := false ;
+    mind_entry_variance :=
+      Option.map (List.map Some) decl.(ind_variance)
+  |}.
 
 
 Section TemplateMonad.
-  Import MonadNotation.
+  Import MCMonadNotation.
 
-  Definition monad_iteri {T} `{Monad T} {A} (f: nat -> A -> T unit) l :=
+  Polymorphic Definition monad_iteri {T} `{Monad T} {A} (f: nat -> A -> T unit) l :=
     monad_map_i f l ;; ret tt.
 
   (** [extract_uniq l fail_msg] returns x if l = [x] or fails with fail_msg *)
-  Definition extract_uniq {A} (l :list A) (fail_msg:string) : TemplateMonad A :=
+  Polymorphic Definition extract_uniq {A} (l :list A) (fail_msg:string) : TemplateMonad A :=
     match l with | (x :: nil)%list => ret x | _ => tmFail fail_msg end.
 
-  Definition get_inductive (id:ident): TemplateMonad inductive :=
-    t <- tmAbout id ;;
-    match t with
-    | Some (IndRef ind) => ret ind
-    | _ => tmFail ("The ident " ++ id ++ " does not refer to an existing inductive ")
+
+  Definition isIndRef := fun x => match x with IndRef _ => true | _ => false end.
+
+  Polymorphic Definition get_inductive@{u} (qid:qualid): TemplateMonad@{_ u} inductive :=
+    ts <- tmLocate qid ;;
+    match List.filter isIndRef ts with
+    | [ IndRef ind ]%list => ret ind
+    | (_ :: _ :: _)%list => tmFail ("Ambiguous definition of " ++ qid ++ " as an inductive")%bs
+    | _ => tmFail ("The ident " ++ qid ++ " does not refer to an existing inductive ")%bs
     end.
 
-  Definition get_const (id:ident) : TemplateMonad kername :=
-    t <- tmAbout id ;;
-    match t with
-    | Some (ConstRef name) => ret name
-    | _ => tmFail ("The ident " ++ id ++ " does not refer to an existing constant")
+  Definition isConstRef := fun x => match x with ConstRef _ => true | _ => false end.
+  Definition get_const (qid:qualid): TemplateMonad kername :=
+    ts <- tmLocate qid ;;
+    match List.filter isConstRef ts with
+    | [ ConstRef kn ]%list => ret kn
+    | (_ :: _ :: _)%list => tmFail ("Ambiguous definition of " ++ qid ++ " as a constant")%bs
+    | _ => tmFail ("The ident " ++ qid ++ " does not refer to an existing const ant")%bs
     end.
 
   Definition assertTM (b:bool) : TemplateMonad unit :=
-    if b then tmFail "assertion failed" else ret tt.
+    if b then tmFail "assertion failed"%bs else ret tt.
 
   (** [def_kername id id_kername] looks up the kernel name of id
       and define a constant with name id_kername to it;
-      fails if there is no associated kernel name*)
+      fails if the associated kernel name is not uniquely defined *)
   Definition def_kername (id id_kername:ident) : TemplateMonad unit :=
-    globref <- tmAbout id ;;
-    kername <- match globref with
-              | Some (ConstRef kn) => ret kn
-              | Some (IndRef ind) => tmEval all (inductive_mind ind)
-              | Some (ConstructRef _ _) =>
-                tmFail ("Found a constructor associated to "++ id ++", no associated kername")
-              | None => tmFail ("No global reference associated to "++id)
+    globrefs <- tmLocate id ;;
+    kername <- match globrefs with
+              | [ConstRef kn]%list => ret kn
+              | [IndRef ind]%list => tmEval all (inductive_mind ind)
+              | [VarRef _]%list =>
+                tmFail ("Found a variable associated to "++ id ++", no associated kername")%bs
+              | [ConstructRef _ _]%list =>
+                tmFail ("Found a constructor associated to "++ id ++", no associated kername")%bs
+              | []%list => tmFail ("No global reference associated to "++id)%bs
+              | (_ :: _ :: _)%list => tmFail ("Multiple global references associated to "++id)%bs
               end ;;
     qkername <- tmQuote kername ;;
     tmMkDefinition id_kername qkername.
