theories/genDiscriminators.v
@@ -1,30 +1,31 @@
-From mathcomp Require Import ssreflect.seq ssreflect.ssrbool.
-From Coq Require Import Strings.String.
+(* From mathcomp Require ssreflect.seq ssreflect.ssrbool. *)
+(* From Coq Require Import Strings.String. *)
 From MetaCoq.Template Require Import All.
 From Genxs Require Import metacoq_utils.
 
 
 Set Primitive Projections.
-Import MonadNotation.
+Import MCMonadNotation.
 
 Section IteriInd.
-  Let ctor_t := (ident × term) × nat.
-  Context (h : inductive -> mutual_inductive_body -> nat -> one_inductive_body -> nat -> ctor_t -> TemplateMonad unit).
+  Universe u.
+  Context (h : inductive -> mutual_inductive_body -> nat -> one_inductive_body -> nat -> constructor_body -> TemplateMonad@{_ u} unit).
 
+  Set Printing Universes.
 
   Definition oneindbody_iteri
            (ind : inductive)
            (mindbody : mutual_inductive_body)
            (oind_index : nat)
            (oindbody : one_inductive_body)
-  : TemplateMonad unit :=
+  : TemplateMonad@{_ u} unit :=
   monad_iteri (h ind mindbody oind_index oindbody) (ind_ctors oindbody).
 
   Definition mutualindbody_iteri (mindname : qualid)
-  : TemplateMonad unit :=
+  : TemplateMonad@{_ u} unit :=
     ind <- get_inductive mindname ;;
-    mindbody <- tmQuoteInductive mindname ;;
-    monad_iteri (oneindbody_iteri ind mindbody) (ind_bodies mindbody).
+    mindbody <- tmQuoteInductive ind.(inductive_mind) ;;
+    monad_iteri (A:= one_inductive_body) (oneindbody_iteri ind mindbody) (ind_bodies mindbody).
 
 End IteriInd.
 
@@ -32,6 +33,7 @@ End IteriInd.
 (** Naming conventions *)
 Section Naming.
   Context (ctor_id : ident).
+  Local Open Scope bs.
 
   Definition discr_id := "is" ++ ctor_id.
   Definition discr_class_id := "is_" ++ ctor_id.
@@ -46,60 +48,69 @@ End Naming.
 
 (** Generation of discrimators *)
 
-Definition qBool :=
-  tInd {| inductive_mind := "Coq.Init.Datatypes.bool"; inductive_ind := 0 |} nil.
+Definition qBool := <% bool %>.
+Definition qtrue := <% true %>.
+Definition qfalse := <% false %>.
 
-Quote Definition qtrue := true.
-Quote Definition qfalse := false.
+(* Definition lf := String (Ascii.ascii_of_nat 10) EmptyString. *)
 
-Definition lf := String (Ascii.ascii_of_nat 10) EmptyString.
+Definition qeq_refl := <% @eq_refl %>.
+Definition qFalse := <% False %>.
+Definition qeq := <% @eq %>.
 
-Definition arguments_string id npars :=
-  let args :=
-    List.fold_left (fun s _ => "{_} " ++ s) (iota 0 npars) "_ : simpl nomatch."
-  in
-  "Arguments " ++ id ++ " " ++ args.
+(* Examples *)
+Definition qisZ := <% fun n : nat => match n with | 0 => true | _ => false end %>.
+Definition qisSuc := <% fun n : nat => match n with | S _ => true | _ => false end %>.
+Definition qisCons := <% fun A (l : list A) => match l with | cons _ _ => true | _ => false end %>.
 
-Quote Definition qeq_refl := @eq_refl.
-Quote Definition qFalse := False.
-Quote Definition qeq := @eq.
+Definition qisEqrefl := <% fun A x y (e : @eq A x y) =>
+                            match e with | eq_refl => true end %>.
+
+
+Definition relNamed (s : string) : aname :=
+  {| binder_name := nNamed s ; binder_relevance := Relevant |}.
 
 Section Builders.
-  Let ctor_t := (ident × term) × nat.
-  Context (indname : qualid)
-           (mindbody : mutual_inductive_body)
-           (oind_index : nat)
-           (oindbody : one_inductive_body)
-           (ctor_index : nat)
-           (* (ctor : ctor_t) *)
-           (* (ctor_id := fst (fst ctor)). *)
-           (ctor_id : ident).
+  Context (ind0 : inductive)
+    (mindbody : mutual_inductive_body)
+    (oindbody : one_inductive_body)
+    (ctor_index : nat)
+    (ctor : constructor_body).
 
   Let npars := ind_npars mindbody.
-  Let ctx := ind_params mindbody.
-  Context (uvs := nil)
-          (ind0 := mkInd indname oind_index)
+  Let param_ctx := ind_params mindbody.
+  Let indices_ctx := ind_indices oindbody.
+
+  Let ctx := app_context param_ctx indices_ctx.
+
+  Context (uvs := nil) (* TODO: manage universes *)
           (ind := fun shift => mkApps_ctx (tInd ind0 uvs) shift ctx).
 
-  Let prop := tSort (Universe.make'' (Level.lProp, false) nil).
-
+  (* to be used with it_mkLambda_or_LetIn;
+     builds the list of variables corresponding to the ctx to be bound
+     shift levels above *)
+  Definition subst_from_ctx (shift : nat) (ctx : context) :=
+    let fold_fun _ '(n, l) := (S n, tRel n :: l)%list in
+    snd (List.fold_right fold_fun (shift , nil) ctx).
 
   (** Building discriminators *)
   Definition build_discriminators :=
-    let discr_id := discr_id ctor_id in
-    let build_branch ctor_k '(((_ , ty),arity): (ident × term) × nat) :=
-      let '(_, tys, _) := decompose_prod ty in
-      let body := if eq_nat ctor_k ctor_index then qtrue else qfalse in
-      (arity, up (build_const (List.skipn npars tys) body))
+    let principal := relNamed "principal"%bs in
+    let case_info0 := mk_case_info ind0 npars Relevant in
+    let boolPred : predicate term :=
+      {| puinst := uvs ;
+         pparams := subst_from_ctx (S (List.length indices_ctx)) param_ctx ;
+         pcontext := (principal :: List.map decl_name indices_ctx)%list ;
+         preturn := <% bool %> |}
     in
-    let brnchs := utils.mapi build_branch (ind_ctors oindbody) in
-    let body := tCase (ind0, npars)
-                      (tLambda (nNamed "z") (ind 1) qBool)
-                      (tRel 0)
-                      brnchs
-    in
-    it_mkLambda_or_LetIn ctx (tLambda (nNamed "z") (ind 0) body).
+    let build_branch ctor_k (cb : constructor_body) : branch term :=
+      {| bcontext := List.map decl_name cb.(cstr_args) ;
+         bbody := if Nat.eqb ctor_k ctor_index then <% true %> else <% false %> |} in
+    let brnchs := mapi build_branch (ind_ctors oindbody) in
+    let body := tCase case_info0 boolPred (tRel 0) brnchs in
+    it_mkLambda_or_LetIn ctx (tLambda principal (ind 0) body).
 
+  (*
   Let pr_name := nNamed "principal".
 
   (** Building discriminator classes *)
@@ -231,41 +242,190 @@ Section Builders.
   (*                         (@Eqdep_dec.UIP_refl_bool tr ispf) *)
   (*   | None => fun H0 : @is_Some A None => @notF (@isSome_pf A None H0) *)
   (*   end). *)
+ *)
+
+  Definition arguments_string id :=
+    let args :=
+      List.fold_left (fun (s:string) _ => ("{_} " ++ s)%bs) ctx "_ : simpl nomatch."%bs
+    in
+    ("Arguments " ++ id ++ " " ++ args)%bs.
+
+  Definition discriminator_notation id :=
+    ("Notation ""'[' '" ++ id++ "' ']'"" := (toSProp " ++ discr_id id ++ ") (format ""[ " ++ id ++ " ]"").")%bs.
 End Builders.
+
 
 Definition gen_from_mind  generate (debug:bool) (mindname : qualid)
   : TemplateMonad unit :=
-  mindbody <- tmQuoteInductive mindname ;;
-  let oid_gen oind_index oindbody :=
-    let ctor_gen ctor_idx ctor :=
-      let '((ctor_id, ty), arity) := ctor in
-      generate debug mindname mindbody oind_index oindbody ctor_idx ctor_id
-    in
+  ind <- get_inductive mindname ;;
+  mindbody <- tmQuoteInductive ind.(inductive_mind) ;;
+  let oid_gen _ oindbody :=
+    ind <- get_inductive oindbody.(ind_name) ;;
+    let ctor_gen := generate debug ind mindbody oindbody in
     monad_iteri ctor_gen (ind_ctors oindbody)
   in
   monad_iteri oid_gen (ind_bodies mindbody).
 
 
 Definition gen_discriminators :=
-  let generate (debug:bool) mindname mindbody oind_index oindbody ctor_idx ctor_id :=
-    let discr_id := discr_id ctor_id in
-    let discr_body := build_discriminators mindname mindbody oind_index oindbody ctor_idx ctor_id in
+  let generate (debug:bool) ind mindbody oindbody ctor_idx ctor :=
+    let discr_id := discr_id ctor.(cstr_name) in
+    let discr_body := build_discriminators ind mindbody oindbody ctor_idx in
     t <- tmEval all discr_body ;;
     if debug then tmPrint t
     else
       tmMkDefinition discr_id t ;;
-      tmMsg (arguments_string discr_id (ind_npars mindbody))
+      tmMsg (arguments_string mindbody oindbody discr_id) ;;
+      tmMsg (discriminator_notation ctor.(cstr_name))
   in
   gen_from_mind generate.
 
+
+From Coq.Logic Require Import StrictProp.
+
+Polymorphic Definition toSProp {X} (p : X -> bool) (x : X) : SProp :=
+  if p x then sUnit else sEmpty.
+
+Module DiscriminatorExamples.
+
+Notation ok := eq_refl.
+Notation oks := stt.
+
+Inductive myBool := myTrue | myFalse.
+MetaCoq Run (gen_discriminators false "myBool"%bs).
+Arguments ismyTrue _ : simpl nomatch.
+Notation "'[' 'myTrue' ']'" := (toSProp ismyTrue) (format "[ myTrue ]").
+Arguments ismyFalse _ : simpl nomatch.
+Notation "'[' 'myFalse' ']'" := (toSProp ismyFalse) (format "[ myFalse ]").
+
+Check oks : [myFalse] myFalse.
+Fail Check oks : [myFalse] myTrue.
+
+Inductive myList (A : Type) := myNil | myCons (hd : A) (tl : myList A) : myList A.
+Arguments myNil {_}.
+Arguments myCons {_} _ _.
+
+MetaCoq Run (gen_discriminators false "myList"%bs).
+
+Arguments ismyNil {_} _ : simpl nomatch.
+Notation "'[' 'myNil' ']'" := (toSProp ismyNil) (format "[ myNil ]").
+Arguments ismyCons {_} _ : simpl nomatch.
+Notation "'[' 'myCons' ']'" := (toSProp ismyCons) (format "[ myCons ]").
+
+
+Check ok : ismyNil (@myNil nat).
+Check ok : ismyCons (myCons 5 myNil).
+Fail Check ok : ismyNil (myCons 5 myNil).
+
+Definition bexfalso {A} (e : false = true) : A :=
+  let B (b : bool) := if b return Type then unit else A in
+  match e in _ = b return B b -> A with
+  | eq_refl => fun x => x
+  end tt.
+
+Definition sexfalso {A} (e : sEmpty) : A := sEmpty_rect (fun _ => A) e.
+
+Definition myCons_hd {A : Type} (l : myList A) : ismyCons l -> A :=
+  match l with
+  | myNil => bexfalso
+  | myCons hd _ => fun _ => hd
+  end.
+
+Definition myCons_hd_s {A : Type} (l : myList A) : [myCons] l -> A :=
+  match l with
+  | myNil => sexfalso
+  | myCons hd _ => fun _ => hd
+  end.
+
+Notation "'[' 'myCons' '-' 'hd' l ']'" :=
+  (myCons_hd_s l ltac:(assumption)) (only parsing).
+Notation "'[' 'myCons' '-' 'hd' l ']'" :=
+  (myCons_hd_s l _) (only printing).
+
+Check fun (l : myList nat) (h : [myCons] l) => Nat.eqb [myCons-hd l] 5.
+
+
+Inductive mySig (A : Type) (B : A -> Type) :=
+  | pair (dfst : A) (dsnd : B dfst) : mySig A B.
+Arguments pair {_ _} _ _.
+
+MetaCoq Run (gen_discriminators false "mySig"%bs).
+Arguments ispair {_} {_} _ : simpl nomatch.
+
+Check ok : ispair (pair 5 (6 : (fun _ => nat) _)).
+
+Notation "'[' 'pair' ']' " := ispair.
+
+Definition pair_dfst (A : Type) (B : A -> Type) (x : mySig A B)
+  : [pair] x -> A :=
+  match x with
+  | pair dfst dsnd => fun _ => dfst
+  end.
+
+Arguments pair_dfst {_} {_} _ _.
+Notation "'[' 'pair' '-' 'dfst' x ']'" :=
+  (pair_dfst x ltac:(assumption)) (only parsing).
+Notation "'[' 'pair' '-' 'dfst' x ']'" :=
+  (pair_dfst x _) (only printing).
+
+Definition pair_dsnd (A : Type) (B : A -> Type) (x : mySig A B)
+  : forall (h : [pair] x), B [pair-dfst x] :=
+  match x with
+  | pair dfst dsnd => fun _ => dsnd
+  end.
+
+Arguments pair_dsnd {_} {_} _ _.
+Notation "'[' 'pair' '-' 'dsnd' x ']'" :=
+  (pair_dsnd x ltac:(assumption + easy)) (only parsing).
+Notation "'[' 'pair' '-' 'dsnd' x ']'" :=
+  (pair_dsnd x _) (only printing).
+
+Eval cbn in let p : mySig nat (fun _ => nat) := pair 5 6 in
+            [pair-dsnd p].
+
+
+Inductive myBoolFam : bool -> Type :=
+  | myIsTrue : myBoolFam true.
+MetaCoq Run (gen_discriminators false "myBoolFam"%bs).
+
+Inductive vect (A : Type) : nat -> Type :=
+| vnil : vect A 0
+| vcons (hd : A) {len_tl} (tl : vect A len_tl) : vect A (S len_tl).
+Arguments vnil {_}.
+Arguments vcons {_} _ {_} _.
+MetaCoq Run (gen_discriminators false "vect"%bs).
+Arguments isvnil {_} {_} _ : simpl nomatch.
+Arguments isvcons {_} {_} _ : simpl nomatch.
+
+Check ok : isvnil (@vnil nat).
+Check ok : isvcons (vcons true vnil).
+Fail Check ok : isvcons (@vnil nat).
+
+
+Inductive even : nat -> Type :=
+| evenZ : even 0
+| evenS {n} (oddn : odd n) : even (S n)
+with odd : nat -> Type :=
+| oddS {n} (evenn : even n) : odd (S n).
+
+MetaCoq Run (gen_discriminators false "even"%bs).
+Arguments isevenZ {_} _ : simpl nomatch.
+Arguments isevenS {_} _ : simpl nomatch.
+Arguments isoddS {_} _ : simpl nomatch.
+
+End DiscriminatorExamples.
+
+
 Definition gen_discr_class :=
-  let generate (debug:bool) mindname mindbody oind_index oindbody ctor_idx ctor_id :=
+  let generate (debug:bool) ind mindbody oind_index oindbody ctor_idx ctor_id :=
     discr_name <- tmEval all (discr_id ctor_id) ;;
     discr_kn <- get_const discr_name;;
-    let discr_class_mid := build_discr_class mindname mindbody oind_index ctor_id discr_kn in
+    let discr_class_mid := build_discr_class ind mindbody ctor_id discr_kn in
     let mindentry := mind_body_to_entry discr_class_mid in
     if debug then
       t <- tmEval all discr_class_mid ;;
+      tmPrint t ;;
+      t <- tmEval all mindentry ;;
       tmPrint t
     else
       tmMkInductive mindentry ;;
@@ -278,11 +438,11 @@ Definition gen_discr_class :=
 
 (** Generation of the type of elimination for the discr class *)
 Definition gen_discr_class_Etype :=
-  let generate (debug:bool) mindname mindbody oind_index oindbody ctor_idx ctor_id :=
+  let generate (debug:bool) ind mindbody oind_index oindbody ctor_idx ctor_id :=
     discrclass_name <- tmEval all (discr_class_id ctor_id) ;;
     discrclass_ind <- get_inductive discrclass_name;;
     let discr_class_Etype :=
-      build_discr_class_Etype mindname mindbody oind_index oindbody ctor_idx (* ctor_id *) (inductive_mind discrclass_ind)
+      build_discr_class_Etype ind mindbody oindbody ctor_idx (* ctor_id *) (inductive_mind discrclass_ind)
     in
     if debug then t <- tmEval all discr_class_Etype ;; tmPrint t
     else
@@ -294,13 +454,13 @@ Definition gen_discr_class_Etype :=
 
 
 Definition gen_discr_class_E :=
-  let generate (debug:bool) mindname mindbody oind_index oindbody ctor_idx ctor_id :=
+  let generate (debug:bool) ind mindbody oind_index oindbody ctor_idx ctor_id :=
     discrclass_name <- tmEval all (discr_class_id ctor_id) ;;
     discrclass_ind <- get_inductive discrclass_name;;
     discrclass_Ety_name <- tmEval all (discr_class_Etype_id ctor_id) ;;
     discrclass_Ety_kn <- get_const discrclass_Ety_name;;
     let discr_class_E :=
-      build_discr_class_E mindname mindbody oind_index oindbody ctor_idx (* ctor_id *) (inductive_mind discrclass_ind) discrclass_Ety_kn
+      build_discr_class_E ind mindbody oindbody ctor_idx (* ctor_id *) (inductive_mind discrclass_ind) discrclass_Ety_kn
     in
     if debug then t <- tmEval all discr_class_E ;; tmPrint t
     else
@@ -313,7 +473,6 @@ Definition gen_discr_class_E :=
 (** Tests *)
 From Coq Require Import ssreflect.
 Module TestGenDiscriminators.
-  Set Primitive Projections.
 
   Inductive myBool := myTrue | myFalse.
   Run TemplateProgram (gen_discriminators false "myBool").
@@ -326,20 +485,185 @@ Module TestGenDiscriminators.
 
   (** Bool *)
   Run TemplateProgram (gen_discriminators false "bool").
-  Arguments istrue _ : simpl nomatch.
-  Arguments isfalse _ : simpl nomatch.
-  Class is_true0 (b:bool) := mkIs_true0 { istrue_pf0 : istrue b }.
-  Run TemplateProgram (t <- tmQuoteInductive "is_true0";; tmPrint t).
-  Run TemplateProgram (gen_discr_class false "bool").
+  (* Arguments istrue _ : simpl nomatch. *)
+  (* Arguments isfalse _ : simpl nomatch. *)
+  (* Class is_true0 (b:bool) := mkIs_true0 { istrue_pf0 : istrue b }. *)
+  (* Run TemplateProgram (t <- tmQuoteInductive "is_true0";; tmPrint t). *)
+  Run TemplateProgram (gen_discr_class true "bool").
   Existing Class is_true.
   Existing Class is_false.
   Run TemplateProgram (gen_discr_class_Etype false "bool").
   Arguments is_true_Etype _ : simpl nomatch.
   Arguments is_false_Etype _ : simpl nomatch.
 
+
   Run TemplateProgram (t <- tmAbout "is_true_Etype";; tmPrint t).
   Run TemplateProgram (s <- tmEval all (discr_class_Etype_id "true") ;; t <- get_const s;; tmPrint t).
-  Run TemplateProgram (gen_discr_class_E false "bool").
+  Run TemplateProgram (gen_discr_class_E true "bool").
+
+  Record T := { t : nat }.
+  Quote Definition Tproj := (fun (x:T) => t x).
+  Run TemplateProgram (t <- tmUnquote Tproj ;; tmPrint t).
+
+  Record T1 (b:bool) := mkT1 { t1 : Datatypes.is_true (istrue b) }.
+  Existing Class T1.
+  Quote Definition T1proj := (fun (x:T1 false) => notF (t1 _ x)).
+
+  Run TemplateProgram (t <- tmUnquote T1proj ;; tmPrint t).
+
+  Check mkIs_true true eq_refl.
+  (* Set Printing All. *)
+  (* Set Printing Universes. *)
+  Quote Definition is_false_E_b2_0 := (* (isfalse_pf true). *)
+    (fun pf_inst (* : is_false true *) =>  @isfalse_pf true pf_inst).
+  Run TemplateProgram (t <- tmUnquote is_false_E_b2_0 ;; tmPrint t).
+
+
+  Quote Definition is_true_E_b2_0 :=
+    (fun (pf_inst : is_true false) => notF (istrue_pf _ pf_inst)).
+
+  Run TemplateProgram (t <- tmUnquote is_true_E_b2_0 ;; tmPrint t).
+
+  Definition is_true_E_b2 :=
+    (tLambda (nNamed "pf_inst")
+            (tApp
+               (tInd
+                  {|
+                  inductive_mind := "Top.TestGenDiscriminators.is_true";
+                  inductive_ind := 0 |} [::])
+               [:: tConstruct
+                     {|
+                     inductive_mind := "Coq.Init.Datatypes.bool";
+                     inductive_ind := 0 |} 1 [::]])
+            (tApp (tConst "Coq.ssr.ssrbool.notF" [::])
+               [:: tProj
+                     ({|
+                      inductive_mind := "Top.TestGenDiscriminators.is_true";
+                      inductive_ind := 0 |}, 1, 0)
+                     (tRel 0)])).
+
+  (* Record is_true (principal : bool) : Prop := mkIs_true *)
+  (*   { istrue_pf : Datatypes.is_true (istrue principal) }. *)
+
+  Run TemplateProgram (t <- tmUnquote is_true_E_b2 ;; tmPrint t).
+  Run TemplateProgram (t <- tmUnquote is_true_E ;; tmPrint t).
+
+(* (tLambda (nNamed "principal") *)
+(*    (tInd {| inductive_mind := "bool"; inductive_ind := 0 |} [::]) *)
+(*    (tCase ({| inductive_mind := "bool"; inductive_ind := 0 |}, 0) *)
+(*       (tRel 0) (tConst "Top.TestGenDiscriminators.is_false_Etype" [::]) *)
+(*       [:: (0, *)
+(*           tLambda (nNamed "pf_inst") *)
+(*             (tApp *)
+(*                (tInd *)
+(*                   {| *)
+(*                   inductive_mind := "Top.TestGenDiscriminators.is_false"; *)
+(*                   inductive_ind := 0 |} [::]) *)
+(*                [:: tConstruct *)
+(*                      {| inductive_mind := "bool"; inductive_ind := 0 |} 0 *)
+(*                      [::]]) *)
+(*             (tApp (tConst "Coq.ssr.ssrbool.notF" [::]) *)
+(*                [:: tProj *)
+(*                      ({| *)
+(*                       inductive_mind := "Top.TestGenDiscriminators.is_false"; *)
+(*                       inductive_ind := 0 |}, 1, 0) *)
+(*                      (tRel 0)])); *)
+(*           (0, *)
+(*           tLambda (nNamed "pf_inst") *)
+(*             (tApp *)
+(*                (tInd *)
+(*                   {| *)
+(*                   inductive_mind := "Top.TestGenDiscriminators.is_false"; *)
+(*                   inductive_ind := 0 |} [::]) *)
+(*                [:: tConstruct *)
+(*                      {| inductive_mind := "bool"; inductive_ind := 0 |} 1 *)
+(*                      [::]]) *)
+(*             (tApp (tConst "Coq.Init.Logic.f_equal" [::]) *)
+(*                [:: tApp *)
+(*                      (tInd *)
+(*                         {| *)
+(*                         inductive_mind := "Coq.Init.Logic.eq"; *)
+(*                         inductive_ind := 0 |} [::]) *)
+(*                      [:: tInd *)
+(*                            {| *)
+(*                            inductive_mind := "Coq.Init.Datatypes.bool"; *)
+(*                            inductive_ind := 0 |} [::]; *)
+(*                          tConstruct *)
+(*                            {| *)
+(*                            inductive_mind := "Coq.Init.Datatypes.bool"; *)
+(*                            inductive_ind := 0 |} 0 [::]; *)
+(*                          tConstruct *)
+(*                            {| *)
+(*                            inductive_mind := "Coq.Init.Datatypes.bool"; *)
+(*                            inductive_ind := 0 |} 0 [::]]; *)
+(*                    tApp *)
+(*                      (tInd *)
+(*                         {| *)
+(*                         inductive_mind := "Top.TestGenDiscriminators.is_false"; *)
+(*                         inductive_ind := 0 |} [::]) *)
+(*                      [:: tConstruct *)
+(*                            {| inductive_mind := "bool"; inductive_ind := 0 |} *)
+(*                            1 [::]]; *)
+(*                    tApp *)
+(*                      (tConstruct *)
+(*                         {| *)
+(*                         inductive_mind := "Top.TestGenDiscriminators.is_false"; *)
+(*                         inductive_ind := 0 |} 0 [::]) *)
+(*                      [:: tConstruct *)
+(*                            {| inductive_mind := "bool"; inductive_ind := 0 |} *)
+(*                            1 [::]; *)
+(*                          tApp *)
+(*                            (tConstruct *)
+(*                               {| *)
+(*                               inductive_mind := "Coq.Init.Logic.eq"; *)
+(*                               inductive_ind := 0 |} 0 [::]) *)
+(*                            [:: tInd *)
+(*                                  {| *)
+(*                                  inductive_mind := "Coq.Init.Datatypes.bool"; *)
+(*                                  inductive_ind := 0 |} [::]; *)
+(*                                tConstruct *)
+(*                                  {| *)
+(*                                  inductive_mind := "Coq.Init.Datatypes.bool"; *)
+(*                                  inductive_ind := 0 |} 0 [::]]]; *)
+(*                    tProj *)
+(*                      ({| *)
+(*                       inductive_mind := "Top.TestGenDiscriminators.is_false"; *)
+(*                       inductive_ind := 0 |}, 1, 0) *)
+(*                      (tRel 0); *)
+(*                    tApp *)
+(*                      (tConstruct *)
+(*                         {| *)
+(*                         inductive_mind := "Coq.Init.Logic.eq"; *)
+(*                         inductive_ind := 0 |} 0 [::]) *)
+(*                      [:: tInd *)
+(*                            {| *)
+(*                            inductive_mind := "Coq.Init.Datatypes.bool"; *)
+(*                            inductive_ind := 0 |} [::]; *)
+(*                          tConstruct *)
+(*                            {| *)
+(*                            inductive_mind := "Coq.Init.Datatypes.bool"; *)
+(*                            inductive_ind := 0 |} 0 [::]]; *)
+(*                    tApp (tConst "Coq.Logic.Eqdep_dec.UIP_refl_bool" [::]) *)
+(*                      [:: tConstruct *)
+(*                            {| *)
+(*                            inductive_mind := "Coq.Init.Datatypes.bool"; *)
+(*                            inductive_ind := 0 |} 0 [::]; *)
+(*                          tProj *)
+(*                            ({| *)
+(*                             inductive_mind := "Top.TestGenDiscriminators.is_false"; *)
+(*                             inductive_ind := 0 |}, 1, 0) *)
+(*                            (tRel 0)]]))])) *)
+
+
+
+
+
+
+
+
+
+
+
 
   Run TemplateProgram (gen_discriminators false "option").
   Class is_none0 {A:Type} (m:option A) := mkIs_None0 { isNone_pf0 : isNone A m }.
